HOL/SepLogic/More_Lists.thy
@@ -1,48 +1,28 @@
 theory More_Lists
-  imports "../DataStrs/Arrays_Ex"
+imports "../DataStrs/Arrays_Ex"
 begin
-
-section {* hd and last *}
-
-lemma hd_conv_nth [rewrite_back]: "length xs > 0 \<Longrightarrow> hd xs = xs ! 0"
-  by (simp add: hd_conv_nth)
-
-lemma last_conv_nth' [rewrite]: "length xs > 0 \<Longrightarrow> last xs = xs ! (length xs - 1)"
-  by (simp add: last_conv_nth)
-
-lemma hd_in_set: "length xs > 0 \<Longrightarrow> hd xs \<in> set xs" by simp
-setup {* add_forward_prfstep_cond @{thm hd_in_set} [with_term "hd ?xs", with_term "set ?xs"] *}
-
-lemma hd_in_mset: "length xs > 0 \<Longrightarrow> hd xs \<in># mset xs" by simp
-setup {* add_forward_prfstep_cond @{thm hd_in_mset} [with_term "hd ?xs", with_term "mset ?xs"] *}
-
-lemma last_in_set: "length xs > 0 \<Longrightarrow> last xs \<in> set xs" by simp
-setup {* add_forward_prfstep_cond @{thm last_in_set} [with_term "last ?xs", with_term "set ?xs"] *}
-
-lemma last_in_mset: "length xs > 0 \<Longrightarrow> last xs \<in># mset xs" by simp
-setup {* add_forward_prfstep_cond @{thm last_in_mset} [with_term "last ?xs", with_term "mset ?xs"] *}
 
 section {* Relationship between mset and set of lists *}
 
 lemma set_butlast [resolve]: "set (butlast xs) \<subseteq> set xs"
   by (simp add: in_set_butlastD subsetI)
 
-theorem mset_butlast [rewrite]: "length xs > 0 \<Longrightarrow> mset (butlast xs) = mset xs - {# last xs #}"
-  by (metis add_diff_cancel_right' append_butlast_last_id length_greater_0_conv list.size(3)
+lemma mset_butlast [rewrite]: "xs \<noteq> [] \<Longrightarrow> mset (butlast xs) = mset xs - {# last xs #}"
+  by (metis add_diff_cancel_right' append_butlast_last_id list.size(3)
       mset.simps(2) size_eq_0_iff_empty size_mset union_code)
 
-theorem insert_mset_to_set [rewrite]: "mset xs' = mset xs + {# x #} \<Longrightarrow> set xs' = set xs \<union> {x}"
+lemma insert_mset_to_set [rewrite]: "mset xs' = mset xs + {# x #} \<Longrightarrow> set xs' = set xs \<union> {x}"
   by (metis set_mset_mset set_mset_single set_mset_union)
 
-theorem delete_mset_to_set [rewrite]:
+lemma delete_mset_to_set [rewrite]:
   "distinct xs \<Longrightarrow> mset xs' = mset xs - {# x #} \<Longrightarrow> set xs' = set xs - {x}"
   by (metis mset_eq_setD mset_remove1 set_remove1_eq)
 
-theorem update_mset_to_set [rewrite]:
+lemma update_mset_to_set [rewrite]:
   "distinct xs \<Longrightarrow> mset xs' = {# y #} + (mset xs - {# x #}) \<Longrightarrow> set xs' = (set xs - {x}) \<union> {y}"
   by (metis insert_mset_to_set mset_remove1 set_remove1_eq union_commute)
 
-theorem mset_update' [rewrite]:
+lemma mset_update' [rewrite]:
   "i < length ls \<Longrightarrow> mset (list_update ls i v) = {#v#} + (mset ls - {# ls ! i #})"
   using mset_update by fastforce
 
